about to change subseq

basic_types.v
@@ -89,33 +89,29 @@ Definition if_z (n: term obj): (term obj) := ppi1 n.
 Lemma if_z_typed n G : tr G (oof n nattp) -> tr G (oof (if_z n) booltp).
 Admitted.
 
-(*n - m*)
-Definition minusbc: (term obj) := lam
-                         (
-                           (*f := 0*)
-                           lam ( (*f:= 1, n := 0*)
-                               lam ((*f := 2, n:= 1, m := 0*)
-                                   let f := (var 2) in
-                                   let n := (var 1) in
-                                   let m := (var 0) in
-                                                  bite (if_z n)
-                                                  (n)
-                                                  (bite (if_z m)
-                                                     (n)
-                                                    (app (app f (app (ppi2 n) triv)) (app (ppi2 m) triv)))
-                                                  ))).
- Definition minus: (term obj) := app theta minusbc.
+(*n1 <= n2*)
+ Definition leq_b n1 := app (wind (lam (* x = 0*)
+                             (lam (*x = 1, y= 0*)
+                                ( lam
+                                    ( (*x = 2, y = 1, z = 0*)
+                                      bite (var 2) (*if n1 = 0*)
+                                           (lam (*x = 3, y = 2, z = 1, n2 = 0*)
+                                             btrue) 
+                                           ( 
+                                             lam
+                                               ( (*x = 3, y = 2, z = 1, n2 = 0*)
+                                                 bite (if_z (var 0))
+                                                      bfalse
+                                                      (app (app (var 1) triv) (app (ppi2 (var 0)) triv))
+                                               )
+                                           )
+                                    )
+                                )
+                             )                           
+                            )) n1.
 
- Lemma minus_typed {G}: tr G (oof minus (arrow nattp (arrow nattp nattp))).
-Admitted.
 
-(*lt_b x y*)
- Definition lt_b := lam ( lam (*x = 1, y = 0*)
-
-                            (if_z (app (app minus (nsucc (var 1)))  (var 0)))
-                       ).
-
-Definition ltb_app m n := app (app lt_b m) n.
+Definition ltb_app n1 n2 := app (leq_b (nsucc n1)) n2.
 
 (*should be fine*)
 Lemma ltapp_typed G m n: tr G (oof m nattp) -> tr G (oof n nattp) ->
@@ -784,3 +780,386 @@ prove_equiv_compat.
 Qed.
 
 
+
+      Definition eqb_sound_fn :=
+    (app (app (app nat_ind_fn (lam
+                  (pi nattp
+                      ( (*x = 1, y = 0*)
+                        arrow 
+                        (equal booltp (app (eq_b (var 1)) (var 0)) btrue
+                               )
+                        (equal nattp (var 1) (var 0))
+                  )
+               )))
+               (lam (*y : nat*)
+                  (lam  (*hyp : eqb 0 y  = tt*)
+                  triv 
+                  )
+               ))
+               (lam (*x : nat*) (lam (*IH: P(x) ie pi y (eqb x y = t -> x = y)*)
+                                   (lam  (*y'  : nat*)
+                                      (lam (*eqb s x y' = t*)
+                                         triv (*s x  = y  : nat*)
+                                      )
+                  )
+               ))).
+     (*          
+  tr
+    [:: hyp_tm
+          (equal booltp
+             (if_z (var 0)) btrue),
+        hyp_tm nattp
+      & G]
+    (deq nzero
+       (var (1 + 0)%coq_nat) nattp) *)
+
+      Lemma bool_contra G J : tr G (deq bfalse btrue booltp) ->
+                          tr G J.
+    Admitted.
+
+      Lemma equal_nzero_help G n:
+        tr G (oof n nattp) -> tr G (oof (lam triv)
+                                       (arrow (equal booltp (if_z n) btrue)
+                                              (equal nattp nzero n)
+                                       )
+                                  ).
+        intros. 
+        replace 
+    (oof (lam triv)
+       (arrow
+          (equal booltp 
+             (if_z n) btrue)
+          (equal nattp nzero n)))
+ with
+            (substj (dot n id) 
+    (oof (lam triv)
+       (arrow
+          (equal booltp 
+             (if_z (var 0)) btrue)
+          (equal nattp nzero (var 0))))) .
+        2:{ simpl. simpsub_big. auto. } 
+        eapply (tr_generalize _ nattp). assumption.
+        apply tr_arrow_intro; auto. { apply tr_equal_formation; auto.
+                                      weaken tr_booltp_formation.
+                                      apply if_z_typed. var_solv'. constructor. }
+                                    { apply tr_equal_formation; auto. var_solv'. }
+                                    simpsub_big.
+        rewrite make_app1. eapply w_elim_hyp.
+        weaken tr_booltp_formation. weaken nat_U01.
+        change triv with (@subst obj (under 1 (dot (ppi2 (var 0)) (dot (ppi1 (var 0)) sh1))) triv). apply tr_sigma_eta_hyp. simpsub_big.
+        simpl. simpsub_big. simpl.
+        rewrite make_app2.
+      match goal with |- tr ?G (deq triv triv ?T) =>
+                      suffices: (tr G (oof (bite (var 2) triv triv) T)) end.
+      { intros Hannoying. constructor. eapply deq_intro. apply Hannoying. }
+      rewrite make_app2.
+        change triv with 
+            (@subst obj (under 2 sh1) triv).
+        apply tr_booltp_eta_hyp; simpl; simpsub_big; simpl.
+        { (*true*)
+          rewrite make_app1.
+          eapply tr_compute_hyp.
+        {
+          constructor. apply equiv_arrow. apply reduce_equiv.
+          apply reduce_bite_beta1. apply reduce_id.
+          apply equiv_refl.
+        }
+        constructor. apply tr_wt_intro. constructor.
+        simpsub_big.
+        eapply tr_compute. { apply equiv_arrow. apply reduce_equiv.
+          apply reduce_bite_beta1. apply reduce_id.
+          apply equiv_refl.
+ } apply equiv_refl. apply equiv_refl.
+        apply (tr_transitivity _#2 (lam (app (subst sh1 (var 1)) (var 0)))).
+        { apply tr_arrow_intro; auto. weaken tr_voidtp_formation.
+          eapply (tr_voidtp_elim  _ (var 0) (var 0)).
+          change voidtp with (@subst obj (sh 1) voidtp). var_solv0.
+        }
+        { apply tr_symmetry. apply tr_arrow_eta.
+          change (arrow voidtp nattp) with (@subst obj (sh 2) (arrow voidtp nattp)).
+          var_solv0.
+        }
+        weaken nat_U01. }
+        {(*false*)
+          eapply (tr_compute_hyp _ [::]).
+        {
+          constructor. apply equiv_equal. apply equiv_refl. apply reduce_equiv.
+          apply reduce_ppi1_beta. apply reduce_id.
+          apply equiv_refl.
+        }
+        apply bool_contra. simpl. apply (deq_intro _#4 (var 0) (var 0)).
+        change (equal booltp bfalse btrue) with (@subst obj sh1 (equal booltp bfalse btrue)).
+        var_solv0. } 
+       Qed. 
+
+
+      Lemma equal_nzero G n:
+        tr G (oof n nattp) ->
+        tr G (deq (if_z n) btrue booltp) ->
+        tr G (deq nzero n nattp).
+        intros.
+        apply (deq_intro _#4 (app (lam triv) triv) (app (lam triv) triv)).
+        apply (tr_arrow_elim _ (equal booltp (if_z n) btrue)).
+        apply tr_equal_formation; auto. weaken tr_booltp_formation.
+        apply if_z_typed. assumption. constructor.
+        apply tr_equal_formation; auto. apply equal_nzero_help. assumption.
+        constructor. assumption. Qed.
+
+  Lemma equal_succ G preds: tr G (oof preds (arrow unittp nattp)) ->
+                        tr G (deq (nsucc (app preds triv )) (ppair bfalse preds) nattp).
+    intros. unfold nsucc. simpsub. apply tr_wt_intro. constructor.
+    simpsub_big.
+    eapply tr_compute. { apply equiv_arrow. apply reduce_equiv.
+                         apply reduce_bite_beta2. apply reduce_id. apply equiv_refl. } apply equiv_refl. apply equiv_refl.
+    apply (tr_transitivity _ _ (lam (app (subst sh1 preds) (var 0)))).
+    {
+            apply tr_arrow_intro; auto.
+            apply (tr_arrow_elim _ unittp); auto.
+            match goal with |- tr ?G (deq ?M ?M ?T) =>
+                                                      change T with
+       (@shift obj 1
+               (arrow unittp nattp)) end. rewrite subst_sh_shift. apply tr_weakening_append1.
+            assumption.
+          apply tr_symmetry. apply tr_unittp_eta.
+          change unittp with (@subst obj (sh 1) unittp). var_solv0.
+    }
+    {
+      apply tr_symmetry. apply tr_arrow_eta. assumption.
+    }
+    weaken nat_U01. Qed.
+
+  Lemma eqb_sound G : tr G (oof eqb_sound_fn (pi nattp (pi nattp (arrow (equal booltp (app (eq_b (var 1)) (var 0))
+                                                                               btrue
+                                                                        )
+                                                                        (equal nattp (var 1) (var 0))
+
+                           )))).
+    unfold eqb_sound_fn.
+    assert (forall G' x, tr G' (oof x nattp) ->
+                    tr G' (oof (pi nattp (arrow (equal booltp (app (eq_b (subst sh1 x)) (var 0))
+                                                                               btrue
+                                                                        )
+                                                                        (equal nattp (subst sh1 x) (var 0))
+
+
+                               ))
+                               U0)
+           ) as Hp.
+    {
+      intros. 
+      apply tr_pi_formation_univ; auto.
+      apply tr_arrow_formation_univ; auto.
+      apply tr_equal_formation_univ; auto.
+      simpsub_big. apply tr_booltp_formation.
+      apply eqapp_typed; try var_solv'.  change nattp with (@subst obj sh1 nattp).
+      rewrite ! subst_sh_shift. apply tr_weakening_append1. assumption.
+      constructor.
+      apply tr_equal_formation_univ; auto; try var_solv'.
+      change nattp with (@subst obj sh1 nattp).
+      rewrite ! subst_sh_shift. apply tr_weakening_append1. assumption.
+    }
+    eapply nat_ind_lamapp; simpsub_big; try reflexivity.
+    { (*type p*)
+      apply tr_arrow_intro; auto. simpsub_big.
+      change (var 1) with (@subst obj sh1 (var 0)). apply Hp; var_solv'. }
+    { (*type BC*)
+       apply tr_pi_intro; auto. 
+       apply tr_arrow_intro; auto. 
+      apply tr_equal_formation; auto.
+      weaken tr_booltp_formation.
+      apply eqapp_typed; auto; try var_solv'. constructor.
+      apply tr_equal_formation; auto; try var_solv'.
+      eapply (tr_compute_hyp _ [::]). constructor. apply equiv_equal. apply equiv_refl.
+      apply eq_b0. apply equiv_refl. simpl. simpsub_big.
+      constructor. apply equal_nzero.
+      var_solv'.
+      apply (deq_intro _#4 (var 0) (var 0)).  
+      match goal with |- tr ?G (deq ?M ?M ?T) => replace T with
+          (subst sh1
+       (equal booltp
+              (if_z (var 0)) btrue)) end.
+      2:{
+        simpl. simpsub_big. auto.
+      }
+      var_solv0.
+    }
+    { (*type IS*)
+       apply tr_pi_intro; auto. 
+       apply tr_arrow_intro; auto.
+       change (var 1) with (@subst obj sh1 (var 0)). weaken Hp.
+       var_solv'.
+       simpl. change (nsucc (var 1)) with (@subst obj sh1 (nsucc (var 0))).
+       weaken Hp. apply nsucc_type. var_solv'.
+       simpsub_big. apply tr_pi_intro; auto.
+       apply tr_arrow_intro; auto.
+      { apply tr_equal_formation; auto.
+      weaken tr_booltp_formation.
+      apply eqapp_typed; auto; try apply nsucc_type; try var_solv'. constructor. }
+      { apply tr_equal_formation; auto; try apply nsucc_type; try var_solv'. }
+      simpsub_big. eapply (tr_compute_hyp _ [::]).
+      { constructor. apply equiv_equal. apply equiv_refl. apply eq_b_succ.
+        apply equiv_refl. }
+      (*split y into pair*)
+      simpl. rewrite make_app1. apply w_elim_hyp. weaken tr_booltp_formation.
+      weaken nat_U01.
+      change triv with (@subst obj (under 1 (dot (ppi2 (var 0))
+                                                 (dot (ppi1 (var 0)) sh1))) triv).
+      apply tr_sigma_eta_hyp.
+      simpsub_big. simpl. simpsub_big.
+      eapply (tr_compute_hyp _ [::]).
+      { constructor. apply equiv_equal. apply equiv_refl.
+        apply equiv_bite. apply reduce_equiv.
+        apply reduce_ppi1_beta. apply reduce_id. apply equiv_refl.
+        apply equiv_app. apply equiv_refl. apply equiv_app.
+        apply reduce_equiv. apply reduce_ppi2_beta. apply reduce_id.
+        apply equiv_refl. apply equiv_refl.
+      }
+      simpl. rewrite make_app2.
+      match goal with |- tr ?G (deq triv triv ?T) =>
+                      suffices: (tr G (oof (bite (var 2) triv triv) T)) end.
+      { intros Hannoying. constructor. eapply deq_intro. apply Hannoying. }
+      change triv with (@subst obj (under 2 sh1) triv).
+      apply tr_booltp_eta_hyp; simpl; simpsub_big.
+      { (*y' = 0*)
+        eapply (tr_compute_hyp _ [::]). { constructor. apply equiv_equal.
+        apply equiv_refl. apply reduce_equiv. apply reduce_bite_beta1.
+        apply reduce_id. apply equiv_refl. }
+        apply bool_contra. simpl. apply (deq_intro _#4 (var 0) (var 0)).
+        change (equal booltp bfalse btrue) with
+            (@subst obj (sh 1) (equal booltp bfalse btrue)). var_solv0. }
+      { (*y' = s y''*)
+       simpl.  eapply (tr_compute_hyp _ [::]).
+          { constructor. apply equiv_equal.
+        apply equiv_refl. apply reduce_equiv. apply reduce_bite_beta2.
+        apply reduce_id. apply equiv_refl. }
+          simpl. rewrite make_app1. eapply tr_compute_hyp.
+          { constructor. apply equiv_arrow. apply reduce_equiv.
+       apply reduce_bite_beta2.
+        apply reduce_id. apply equiv_refl. }
+          simpl.
+          constructor.
+          eapply (tr_transitivity _#2 (nsucc (app (var 1) triv))).
+          { (*succ x = succ (y' * *)
+            apply nsucc_type.
+            apply (deq_intro _#4 (app (app (var 2) (app (var 1) triv))
+                                      (var 0))
+                             (app (app (var 2) (app (var 1) triv))
+                                      (var 0))
+                  ).
+            apply (tr_arrow_elim _
+(equal booltp (app (eq_b (var 3)) (app (var 1) triv))
+       btrue)).
+      { apply tr_equal_formation; auto.
+      weaken tr_booltp_formation.
+      apply eqapp_typed; auto; try apply nsucc_type; try var_solv'.
+      apply (tr_arrow_elim _ unittp); auto.
+      change 
+          (arrow unittp nattp) with (@subst obj (sh 2)
+(arrow unittp nattp)
+                                    ). var_solv'. constructor. constructor. }
+      {
+        apply tr_equal_formation; auto; try var_solv'.
+        apply (tr_arrow_elim _ unittp); auto.
+      change 
+          (arrow unittp nattp) with (@subst obj (sh 2)
+(arrow unittp nattp)
+                                    ). var_solv'. constructor. 
+      }
+      match goal with |- tr ?G (deq ?M ?M ?T) => change T with
+          (subst1 (app (var 1) triv)
+       (arrow
+          (equal booltp
+             (app (eq_b (var 4))
+                (var 0)) btrue)
+          (equal nattp (var 4) (var 0)))) end.
+      apply (tr_pi_elim _ nattp).
+      match goal with |- tr ?G (deq ?M ?M ?T) => change T with
+      ( subst (sh 3) (pi nattp
+          (arrow
+             (equal booltp
+                (app (eq_b (var 1)) (var 0)) btrue)
+             (equal nattp (var 1) (var 0))))) end. var_solv'.
+        apply (tr_arrow_elim _ unittp); auto.
+      change 
+          (arrow unittp nattp) with (@subst obj (sh 2)
+(arrow unittp nattp)
+                                    ). var_solv'. constructor.
+      match goal with |- tr ?G (deq ?M ?M ?T) => change T with
+          (subst (sh 1)
+       (equal booltp
+          (app (eq_b (var 2)) (app (var 0) triv))
+          btrue)) end. var_solv'. }
+          {  apply equal_succ.
+      change 
+          (arrow unittp nattp) with (@subst obj (sh 2)
+(arrow unittp nattp)
+                                    ). var_solv'.  } } } 
+Qed.
+
+Lemma eqb_P G n m : tr G (oof n nattp) ->
+                    tr G (oof m nattp) ->
+  tr G (deq (app (eq_b n) m) btrue booltp) ->
+                    tr G (deq n m nattp).
+  intros.
+  match goal with |- tr G ?J => replace J with (substj (dot triv id)
+                                                    (deq (subst (sh 1) n)
+                                                         (subst (sh 1) m)
+                                                    nattp)
+                                             ) end.
+  2:{
+    unfold substj. simpsub. auto.
+  }
+  eapply tr_generalize. apply tr_equal_intro in H1. apply H1.
+  remember (subst (sh 1) n) as n'.
+  remember (subst (sh 1) m) as m'.
+  suffices: (tr (hyp_tm (equal booltp (app (eq_b n) m) btrue) :: G)
+                (deq triv (app (app (app eqb_sound_fn n') m') (var 0))
+                       (equal nattp n' m')
+            )).
+  move/ tr_eq_reflexivity => Hdeq.
+  constructor. assumption.
+  apply tr_symmetry. apply tr_equal_eta.
+  assert (tr
+    (hyp_tm (equal booltp (app (eq_b n) m) btrue)
+     :: G) (deq n' n' nattp)) as Hn. 
+    subst; change nattp with (@subst obj (sh 1) nattp);
+      rewrite ! subst_sh_shift; apply tr_weakening_append1; assumption.
+  assert (tr
+    (hyp_tm (equal booltp (app (eq_b n) m) btrue)
+     :: G) (deq m' m' nattp)) as Hm. 
+  subst; change nattp with (@subst obj (sh 1) nattp);
+      rewrite ! subst_sh_shift; apply tr_weakening_append1; assumption.
+ (* replace (equal nattp n' m') with
+      (subst1 (var 0) (equal nattp (subst (sh 1) n') (subst (sh 1) m'))). *)
+  apply (tr_arrow_elim _ (equal booltp (app (eq_b n') m') btrue)
+        ).
+  - apply tr_equal_formation. weaken tr_booltp_formation.
+    apply eqapp_typed; assumption.
+    constructor. apply tr_equal_formation; auto.
+    - match goal with |- tr ?G (deq ?M ?M ?T) => replace T with  
+          (subst1 m' 
+       (arrow
+          (equal booltp (app (eq_b (subst (sh 1) n')) (var 0)) btrue)
+          (equal nattp (subst (sh 1) n') (var 0)))) end.
+      2:{
+        unfold subst1. simpsub_big.  auto.
+      }
+      apply (tr_pi_elim _ nattp).
+      match goal with |- tr ?G (deq ?M ?M ?T) => replace T with
+       (subst1 n' (pi nattp
+          (arrow
+             (equal booltp
+                (app
+                   (eq_b (var 1))
+                   (var 0)) btrue)
+             (equal nattp  (var 1)
+                (var 0))))) end.
+      apply (tr_pi_elim _ nattp); try assumption. apply eqb_sound.
+      simpsub_big. auto.
+      assumption.
+      match goal with |- tr ?G (deq ?M ?M ?T) => replace T with
+      (subst (sh 1) (equal booltp (app (eq_b n) m) btrue)) end. var_solv0.
+      subst. simpsub_big. auto.
+Qed.
+
+(*write out subseq refl and subseq trans on paper*)
